Cleaned up proofs a bunch

Vector.thy
@@ -3,7 +3,8 @@ imports Main
 begin
 
 fun insert_at :: "nat \<Rightarrow> 'a \<Rightarrow> 'a list \<Rightarrow> 'a list" where
-  "insert_at 0 a' as = a' # as"
+  "insert_at 0 a' [] = a' # []"
+| "insert_at 0 a' (a # as) = a' # a # as"
 | "insert_at (Suc x) a' [] = undefined"
 | "insert_at (Suc x) a' (a # as) = a # insert_at x a' as"
 
@@ -15,18 +16,25 @@ fun lookup :: "nat \<Rightarrow> 'a list \<Rightarrow> 'a option" where
 lemma [simp]: "x \<le> length as \<Longrightarrow> length (insert_at x a as) = Suc (length as)"
   by (induction x a as rule: insert_at.induct) simp_all
 
+lemma [simp]: "x \<le> length as \<Longrightarrow> y \<le> x \<Longrightarrow> 
+    insert_at y b (insert_at x a as) = insert_at (Suc x) a (insert_at y b as)"
+  proof (induction x a as arbitrary: y rule: insert_at.induct) 
+  case 4
+    thus ?case by (induction y) simp_all
+  qed simp_all
+
 lemma [simp]: "x \<le> length as \<Longrightarrow> lookup x (insert_at x a as) = Some a"
   by (induction x a as rule: insert_at.induct) simp_all
 
 lemma [simp]: "x \<le> length as \<Longrightarrow> y < x \<Longrightarrow> lookup y (insert_at x a as) = lookup y as"
   proof (induction x a as arbitrary: y rule: insert_at.induct)
-  case 3
+  case 4
     thus ?case by (induction y) simp_all
   qed simp_all
 
 lemma [simp]: "x \<le> length as \<Longrightarrow> x \<le> y \<Longrightarrow> lookup (Suc y) (insert_at x a as) = lookup y as"
   proof (induction x a as arbitrary: y rule: insert_at.induct)
-  case 3
+  case 4
     thus ?case by (induction y) simp_all
   qed simp_all
 
